rebuilding ordinals is weakening

theories/Logic/PA_omega.v
@@ -73,7 +73,7 @@ Inductive PA_omega_theorem : formula -> nat -> ord -> Type :=
 | weakening : forall (A D : formula) (d : nat) (alpha : ord),
     closed A = true ->
     PA_omega_theorem D d alpha ->
-    PA_omega_theorem (lor A D) d (ord_succ alpha)
+    PA_omega_theorem (lor A D) d (ord_succ (ord_add alpha (nat_ord (num_conn A))))
 
 | demorgan1 : forall (A B : formula) (d1 d2 : nat)
                      (alpha1 alpha2 : ord),
@@ -110,12 +110,12 @@ Inductive PA_omega_theorem : formula -> nat -> ord -> Type :=
 | w_rule1 : forall (A : formula) (n : nat) (d : nat) (alpha : ord)
   (g : forall (m : nat),
       PA_omega_theorem (substitution A n (represent m)) d alpha),
-  PA_omega_theorem (univ n A) d (cons alpha 0 Zero)
+  PA_omega_theorem (univ n A) d (ord_succ alpha)
 
 | w_rule2 : forall (A D : formula) (n : nat) (d : nat) (alpha : ord)
   (g : forall (m : nat),
     PA_omega_theorem (lor (substitution A n (represent m)) D) d alpha),
-  PA_omega_theorem (lor (univ n A) D) d (cons alpha 0 Zero)
+  PA_omega_theorem (lor (univ n A) D) d (ord_succ alpha)
 
 | cut1 : forall (C A : formula) (d1 d2 : nat) (alpha1 alpha2 : ord),
     PA_omega_theorem (lor C A) d1 alpha1 ->
@@ -171,9 +171,9 @@ apply eval_represent.
 Qed.
 
 Lemma w_rule_exmp : forall (n : nat),
-  PA_omega_theorem (univ n (atom (equ (var n) (var n)))) 0 (cons Zero 0 Zero).
+  PA_omega_theorem (univ n (atom (equ (var n) (var n)))) 0 (ord_succ Zero).
 Proof.
-intros. 
+intros.
 apply w_rule1. simpl. rewrite eq_nat_refl. apply equ_refl.
 Qed.
 
@@ -217,8 +217,7 @@ Lemma ord_nf : forall (A : formula) (d : nat) (alpha : ord),
 Proof.
 intros. induction H; try apply ord_succ_nf; try apply ord_max_nf; auto.
 - apply zero_nf.
-- apply single_nf. apply (H 0).
-- apply single_nf. apply (H 0).
+- apply nf_add; auto. apply nf_nat.
 Qed.
 
 Lemma ord_monot : forall (A : formula) (d : nat) (alpha beta : ord),
@@ -371,18 +370,16 @@ apply eval_closed. apply eval_represent.
 Qed.
 
 
-
-
-
-
 Lemma LEM_atomic : forall (a : atomic_formula),
   closed_a a = true ->
-  PA_omega_theorem (lor (neg (atom a)) (atom a)) 0 (ord_succ Zero).
+  PA_omega_theorem (lor (neg (atom a)) (atom a)) 0 (ord_succ (ord_succ Zero)).
 Proof.
 intros.
 destruct (correctness_decid a H) as [H0 | H0].
-- apply weakening; auto. apply axiom. apply H0.
-- apply exchange1. apply weakening; auto. apply axiom. apply H0.
+- assert (ord_succ (ord_add Zero (nat_ord (num_conn (neg (atom a))))) = ord_succ (ord_succ Zero)). auto.
+  destruct H1. apply weakening; auto. apply axiom. apply H0.
+- apply exchange1. assert (ord_succ (ord_add Zero (nat_ord (num_conn (atom a)))) = ord_succ Zero). auto.
+  apply (ord_incr _ _ (ord_succ Zero)). destruct H1. apply weakening; auto. apply axiom. apply H0. apply ord_succ_monot. repeat apply ord_succ_nf. apply Zero_nf.
 Qed.
 
 (*
@@ -398,7 +395,7 @@ by strong induction on n, the number of connectives.
 *)
 
 Definition P1 (A : formula) : Type :=
-  closed A = true -> PA_omega_theorem (lor (neg A) A) 0 (ord_succ (w_tower ((num_conn A) + (num_conn A)))).
+  closed A = true -> PA_omega_theorem (lor (neg A) A) 0 (ord_succ (ord_succ (nat_ord ((num_conn A) + (num_conn A))))).
 
 Definition P2 (A : formula) (n : nat) : Type :=
   num_conn A = n -> P1 A.
@@ -410,10 +407,7 @@ Lemma P3_0 : P3 0.
 Proof.
 unfold P3, P2. intros.
 destruct A as [a | | | ].
-- unfold P1. intros. apply (ord_incr _ _ (cons Zero 0 Zero)). 
-  + apply LEM_atomic. auto.
-  + simpl. apply ord_ltb_lt. auto.
-  + apply ord_succ_nf. simpl. apply single_nf. apply Zero_nf. 
+- unfold P1. intros. apply LEM_atomic. auto.
 - inversion H.
 - inversion H.
 - inversion H.
@@ -450,12 +444,10 @@ unfold P3,P2,P1. intros.
 destruct A as [a | B | B C | m B].
 - inversion H0.
 - inversion H0. pose proof (H n (leq_refl n) B H3 H1).
-  apply (ord_incr _ _ (ord_succ (ord_succ (w_tower ((num_conn B) + (num_conn B)))))).
+  apply (ord_incr _ _ (ord_succ (ord_succ (ord_succ (nat_ord ((num_conn B) + (num_conn B))))))).
   + apply negation2. apply exchange1. apply H2.
-  + apply ord_lt_succ. unfold num_conn. fold num_conn. destruct (num_conn B).
-    * simpl. apply ord_ltb_lt. auto.
-    * apply ord_ltb_lt. apply (ord_ltb_trans _ _ _ (ord_lt_ltb _ _ (w_tower_succ _))). apply ord_lt_ltb. apply w_tower_lt. lia.
-  + apply ord_succ_nf. apply w_tower_nf.
+  + apply ord_lt_succ. unfold num_conn. fold num_conn. repeat rewrite ord_succ_nat. apply nat_ord_lt. lia.
+  + repeat apply ord_succ_nf. apply nf_nat.
 
 - destruct (closed_lor _ _ H1) as [HB HC].
   destruct (num_conn_lor _ _ _ H0) as [HB' HC'].
@@ -464,21 +456,31 @@ destruct A as [a | B | B C | m B].
   pose proof (H (num_conn C) HC' C (eq_refl (num_conn C)) HC).
   apply (weakening B _ _ _ HB) in H3. apply exchange1 in H3. apply exchange2 in H3. apply associativity1 in H3.
   pose proof (demorgan2 B C (lor B C) 0 0 _ _ H2 H3).
-  apply (ord_incr _ _ (ord_succ (ord_max (ord_succ (ord_succ (w_tower ((num_conn B)+ (num_conn B))))) (ord_succ (ord_succ (w_tower ((num_conn C) + (num_conn C)))))))).
-  + apply H4.
-  + unfold num_conn. fold num_conn. apply ord_lt_succ. apply ord_ltb_lt. apply (ord_ltb_trans _ _ _ (ord_lt_ltb _ _ (w_tower_max _ _))). apply ord_lt_ltb. apply w_tower_lt. lia.
-  + apply ord_succ_nf. apply w_tower_nf.
-
+  case (num_conn C) eqn:X.
+  + case (num_conn B) eqn:X1.
+    * unfold num_conn in *. fold num_conn in *. rewrite plus_n_0 in *. rewrite <- plus_n_Sm in *. rewrite <- ord_succ_nat in *. rewrite plus_comm. rewrite <- plus_n_Sm in *. rewrite <- ord_succ_nat in *.
+      rewrite ord_add_zero in H4. repeat rewrite ord_max_succ_succ in H4. rewrite X,X1. repeat rewrite plus_n_0 in *. rewrite ord_max_lem2 in H4. apply H4. apply ord_ltb_irrefl.
+    * unfold num_conn in *. fold num_conn in *. rewrite X,X1. rewrite plus_n_0 in *. repeat rewrite <- plus_n_Sm in *. repeat rewrite ord_succ_nat in *.
+      repeat rewrite <- ord_add_nat in H4. rewrite plus_n_0 in *. rewrite <- ord_succ_nat in *. repeat rewrite ord_max_succ_succ in H4; try rewrite plus_n_0 in *; rewrite ord_max_lem2 in H4; try apply H4;
+      repeat rewrite ord_succ_nat; try apply nf_nat; apply ltb_asymm; apply ord_lt_ltb; repeat rewrite <- ord_add_nat; apply nat_ord_lt; lia.
+  + case (num_conn B) eqn:X1.
+    * unfold num_conn in *. fold num_conn in *. rewrite X,X1. unfold add in *. fold add in *. repeat rewrite <- plus_n_Sm in *. repeat rewrite ord_succ_nat in *.
+      repeat rewrite <- ord_add_nat in H4. rewrite plus_n_0 in *. rewrite <- ord_succ_nat in *. repeat rewrite ord_max_succ_succ in H4. rewrite ord_max_symm in H4. rewrite ord_max_lem2 in H4; try apply H4;
+      repeat rewrite ord_succ_nat; try apply nf_nat; apply ltb_asymm; apply ord_lt_ltb; repeat rewrite <- ord_add_nat; apply nat_ord_lt; lia.
+    * unfold num_conn in *; fold num_conn in *; rewrite X,X1 in *; unfold add in *; fold add in *; repeat rewrite <- plus_n_Sm in *; repeat rewrite ord_succ_nat in *;
+      repeat rewrite <- ord_add_nat in *; repeat rewrite ord_max_succ_succ in H4; repeat rewrite <- plus_n_Sm in *; rewrite plus_assoc; rewrite plus_comm;
+      rewrite plus_assoc; rewrite <- plus_n_Sm; rewrite (plus_comm n0 _); rewrite plus_comm; rewrite <- plus_n_Sm; rewrite plus_assoc; rewrite plus_assoc; rewrite <- (plus_assoc _ n0 n0); rewrite plus_n_Sm; rewrite plus_n_Sm; rewrite plus_comm; repeat rewrite plus_n_Sm in *. rewrite plus_comm in H4.
+      case (ord_ltb (nat_ord (S n0 + (n1 + S (S (S (S n1)))))) (nat_ord (n0 + S (S (S (S n0))) + S n1))) eqn:X2.
+      --  rewrite ord_max_lem1 in H4; auto. apply (ord_incr _ _ _ _ H4).
+          ++  repeat rewrite ord_succ_nat. apply nat_ord_lt. lia.
+          ++  apply nf_nat.
+      --  rewrite ord_max_lem2 in H4; auto. apply (ord_incr _ _ _ _ H4).
+          ++  repeat rewrite ord_succ_nat. apply nat_ord_lt. lia.
+          ++  apply nf_nat.
 - inversion H0. apply exchange1.
-  apply (ord_incr _ _ (w_tower ((num_conn (univ m B))+(num_conn (univ m B))))).
-  + unfold num_conn. fold num_conn. rewrite <- plus_n_Sm. apply w_rule2. fold w_tower. intros k.
-    destruct H3. pose proof (H _ (leq_refl _) _ (num_conn_sub _ _ _) (closed_univ_sub _ _ H1 _ (eval_closed _ (eval_represent k)))).
-    rewrite num_conn_sub in H2. apply (ord_incr _ _ (ord_succ (ord_succ (w_tower ((num_conn B) + (num_conn B)))))).
-    * apply exchange1. apply (quantification2 _ _ _ (represent k)). apply repr_closed. apply H2.
-    * apply w_tower_succ2.
-    * apply w_tower_nf.
-  + apply ord_succ_monot.
-  + apply ord_succ_nf. apply w_tower_nf.
+  unfold num_conn. fold num_conn. rewrite <- plus_n_Sm. rewrite <- ord_succ_nat. rewrite plus_comm. rewrite <- plus_n_Sm. rewrite <- ord_succ_nat.
+  apply w_rule2. intros k. destruct H3. pose proof (H _ (leq_refl _) _ (num_conn_sub _ _ _) (closed_univ_sub _ _ H1 _ (eval_closed _ (eval_represent k)))).
+  rewrite num_conn_sub in H2. apply exchange1. apply (quantification2 _ _ _ (represent k)). apply repr_closed. apply H2.
 Qed.
 
 Lemma P3_lemma : forall n, P3 n.
@@ -497,7 +499,7 @@ Qed.
 
 Lemma LEM : forall (A : formula),
   closed A = true ->
-  PA_omega_theorem (lor (neg A) A) 0 (ord_succ (w_tower ((num_conn A)+(num_conn A)))).
+  PA_omega_theorem (lor (neg A) A) 0 (ord_succ (ord_succ (nat_ord ((num_conn A)+(num_conn A))))).
 Proof. intros. apply (P1_lemma A H). Qed.
 
 
@@ -604,7 +606,7 @@ Lemma LEM_term_atomic :
     free_list_a a = [n] ->
     PA_omega_theorem (lor (neg (atom (substitution_a a n s)))
                           (atom (substitution_a a n t)))
-                      0 (ord_succ Zero).
+                      0 (ord_succ (ord_succ Zero)).
 Proof.
 intros a n s t H Ha.
 destruct (correctness_decid (substitution_a a n s)) as [H0 | H0].
@@ -614,11 +616,15 @@ destruct (correctness_decid (substitution_a a n s)) as [H0 | H0].
 - pose proof (correct_closed _ H0) as HC.
   pose proof (LEM_term_atomic' s t a n H). apply H1 in H0.
   apply axiom in H0. unfold substitution in H0.
-  apply weakening; auto.
-- apply exchange1. apply weakening; auto.
+  assert (ord_succ (ord_add Zero (nat_ord (num_conn (neg (substitution (atom a) n s))))) = ord_succ (ord_succ Zero)). auto.
+  destruct H2. apply weakening; auto.
+- apply exchange1. assert (ord_succ (ord_add Zero (nat_ord (num_conn (substitution (atom a) n t)))) = (ord_succ Zero)). auto.
+  apply (ord_incr _ _ (ord_succ Zero)). destruct H1. unfold substitution. apply weakening; auto.
   + simpl. apply (incorrect_subst_closed a n s t); auto.
     apply eval_closed. destruct (correct_eval s t H). apply H2.
   + apply axiom. apply H0.
+  + apply ord_succ_monot.
+  + repeat apply ord_succ_nf. apply zero_nf.
 Qed.
 
 
@@ -631,7 +637,7 @@ Definition Q1 (A : formula) : Type := forall (n : nat) (s t : term),
   correct_a (equ s t) = true ->
   free_list A = [n] ->
   PA_omega_theorem (lor (neg (substitution A n s)) (substitution A n t))
-                   0 (ord_succ (w_tower ((num_conn A)+(num_conn A)))).
+                   0 (ord_succ (ord_succ (nat_ord ((num_conn A)+(num_conn A))))).
 
 Definition Q2 (A : formula) (n : nat) : Type := num_conn A = n -> Q1 A.
 
@@ -662,8 +668,7 @@ Lemma Q3_0 : Q3 0.
 Proof.
 unfold Q3, Q2. intros.
 destruct A as [a | | | ].
-- unfold Q1. intros. apply (ord_incr _ _ (ord_succ Zero)). apply LEM_term_atomic; auto.
-  apply ord_lt_succ. apply zero_lt. apply ord_succ_nf. apply w_tower_nf.
+- unfold Q1. intros. apply LEM_term_atomic; auto.
 - inversion H.
 - inversion H.
 - inversion H.
@@ -676,53 +681,83 @@ unfold Q3,Q2,Q1. intros.
 destruct A as [| B | B C | m B].
 - inversion H0.
 - inversion H0. apply negation2. fold substitution. apply exchange1. unfold num_conn. fold num_conn.
-  apply (ord_incr _ _ (ord_succ (w_tower ((num_conn B)+(num_conn B))))).
-  apply (H n (leq_refl n) B H4 n0 t s); auto. apply equ_symm,H1.
-  apply ord_ltb_lt. apply (ord_ltb_trans _ _ _ (ord_lt_ltb _ _ (w_tower_succ _))). apply ord_lt_ltb. apply w_tower_lt. lia.
-  apply single_nf. apply w_tower_nf.
+  apply (ord_incr _ _ (ord_succ (ord_succ (nat_ord ((num_conn B)+(num_conn B)))))).
+  + apply (H n (leq_refl n) B H4 n0 t s); auto. apply equ_symm,H1.
+  + repeat rewrite ord_succ_nat. apply nat_ord_lt. lia.
+  + apply ord_succ_nf. apply nf_nat.
 - destruct (free_list_lor B C n0 H2) as [HB HC].
   destruct (num_conn_lor _ _ _ H0) as [HB' HC'].
   destruct (correct_closed_t _ _ H1) as [Hs Ht].
-  apply (ord_incr _ _ (ord_succ (ord_max (ord_succ (ord_succ (w_tower ((num_conn B) + (num_conn B))))) (ord_succ (ord_succ (w_tower ((num_conn C)+(num_conn C)))))))).
-  + apply (demorgan2 _ _ _ 0 0 (ord_succ (ord_succ (w_tower ((num_conn B) + (num_conn B))))) (ord_succ (ord_succ (w_tower ((num_conn C)+(num_conn C)))))).
+  case (num_conn C) eqn:X.
+  + unfold num_conn in *. fold num_conn in *. rewrite X in *. rewrite plus_n_0.
+    assert ((ord_succ (ord_succ (nat_ord (S (num_conn B) + S (num_conn B))))) = (ord_succ (ord_succ (ord_max (ord_succ (ord_succ (nat_ord (num_conn B + num_conn B)))) (ord_succ (ord_succ (nat_ord (num_conn C + num_conn C)))))))).
+    { rewrite X. rewrite plus_n_0. repeat rewrite ord_max_succ_succ. rewrite ord_max_lem2. repeat rewrite ord_succ_nat. repeat rewrite plus_n_Sm. rewrite plus_comm at 1. rewrite <- plus_n_Sm. rewrite plus_comm. rewrite plus_n_Sm. auto. case (nat_ord (num_conn B + num_conn B)); auto. }
+    rewrite H3. apply (demorgan2 _ _ _ 0 0 (ord_succ (ord_succ (nat_ord ((num_conn B)+(num_conn B))))) (ord_succ (ord_succ (nat_ord ( (num_conn C)+(num_conn C)))))).
     * apply associativity1. apply exchange1. apply weakening.
-      { destruct HC as [HC | HC].
-        { apply (one_var_free_lemma _ _ _ Ht HC). }
-        { rewrite closed_subst_eq; apply HC. }
-        }
-      { destruct HB as [HB | HB].
-        { apply (H (num_conn B) HB' B (eq_refl (num_conn B)) n0 s t H1 HB). }
-        { rewrite closed_subst_eq, closed_subst_eq; auto. apply (LEM B HB). }
-        }
-      * apply associativity1. apply exchange2. apply exchange1. apply weakening.
-      { destruct HB as [HB | HB].
-        { apply (one_var_free_lemma _ _ _ Ht HB). }
-        { rewrite closed_subst_eq; apply HB. }
-        }
-      { destruct HC as [HC | HC].
-        { apply (H (num_conn C) HC' C (eq_refl (num_conn C)) n0 s t H1 HC). }
-        { rewrite closed_subst_eq, closed_subst_eq; auto. apply (LEM C HC). }
-        }
-  + unfold num_conn. fold num_conn. apply ord_lt_succ. apply ord_ltb_lt. apply (ord_ltb_trans _ _ _ (ord_lt_ltb _ _ (w_tower_max _ _))). apply ord_lt_ltb. apply w_tower_lt. lia.
-  + apply ord_succ_nf. apply w_tower_nf.
+      --  destruct HC as [HC | HC].
+          ++  apply (one_var_free_lemma _ _ _ Ht HC).
+          ++  rewrite closed_subst_eq; apply HC.
+      --  destruct HB as [HB | HB].
+          ++  destruct X. apply (H (num_conn B) HB' B (eq_refl (num_conn B)) n0 s t H1 HB).
+          ++  rewrite closed_subst_eq, closed_subst_eq; auto. apply (LEM B HB).
+    * apply associativity1. apply exchange2. apply exchange1. apply weakening.
+      --  destruct HB as [HB | HB].
+          ++ apply (one_var_free_lemma _ _ _ Ht HB).
+          ++ rewrite closed_subst_eq; apply HB.
+      --  destruct HC as [HC | HC].
+          ++  destruct X. apply (H (num_conn C) HC' C (eq_refl (num_conn C)) n0 s t H1 HC).
+          ++  rewrite closed_subst_eq, closed_subst_eq; auto. apply (LEM C HC).
+  + case (num_conn B) eqn:X1.
+    * unfold num_conn in *. fold num_conn in *. rewrite X1 in *. unfold add at 2. unfold add at 2.
+      assert ((ord_succ (nat_ord (S (num_conn C) + S (num_conn C)))) = ord_succ (ord_max (ord_succ (ord_succ (nat_ord (num_conn B + num_conn B)))) (ord_succ (ord_succ (nat_ord (num_conn C + num_conn C)))))).
+      { rewrite X1. unfold add at 2. unfold nat_ord at 2. repeat rewrite ord_max_succ_succ. rewrite ord_max_symm. rewrite ord_max_lem2. repeat rewrite ord_succ_nat. repeat rewrite plus_n_Sm. rewrite plus_comm at 1. rewrite <- plus_n_Sm. rewrite plus_comm. rewrite plus_n_Sm. auto. case (nat_ord (num_conn C + num_conn C)); auto. }
+      rewrite H3. apply (demorgan2 _ _ _ 0 0 (ord_succ (ord_succ (nat_ord ((num_conn B)+(num_conn B))))) (ord_succ (ord_succ (nat_ord ( (num_conn C)+(num_conn C)))))).
+      --  apply associativity1. apply exchange1. apply weakening.
+          ++  destruct HC as [HC | HC].
+              **  apply (one_var_free_lemma _ _ _ Ht HC).
+              **  rewrite closed_subst_eq; apply HC.
+          ++  destruct HB as [HB | HB].
+              **  destruct X,X1. apply (H (num_conn B) HB' B (eq_refl (num_conn B)) n0 s t H1 HB).
+              **  rewrite closed_subst_eq, closed_subst_eq; auto. apply (LEM B HB).
+      --  apply associativity1. apply exchange2. apply exchange1. apply weakening.
+          ++  destruct HB as [HB | HB].
+              ** apply (one_var_free_lemma _ _ _ Ht HB).
+              ** rewrite closed_subst_eq; apply HB.
+          ++  destruct HC as [HC | HC].
+              **  destruct X,X1. apply (H (num_conn C) HC' C (eq_refl (num_conn C)) n0 s t H1 HC).
+              **  rewrite closed_subst_eq, closed_subst_eq; auto. apply (LEM C HC).
+    * apply (ord_incr _ _ (ord_succ (ord_max (ord_succ (ord_succ (nat_ord ((num_conn B) + (num_conn B))))) (ord_succ (ord_succ (nat_ord ((num_conn C)+(num_conn C)))))))).
+      --  apply (demorgan2 _ _ _ 0 0 (ord_succ (ord_succ (nat_ord ((num_conn B) + (num_conn B))))) (ord_succ (ord_succ (nat_ord ((num_conn C)+(num_conn C)))))).
+          ++  apply associativity1. apply exchange1. apply weakening.
+              **  destruct HC as [HC | HC].
+                  { apply (one_var_free_lemma _ _ _ Ht HC). }
+                  { rewrite closed_subst_eq; apply HC. }
+              **  destruct X,X1. destruct HB as [HB | HB].
+                  { apply (H (num_conn B) HB' B (eq_refl (num_conn B)) n0 s t H1 HB). }
+                  { rewrite closed_subst_eq, closed_subst_eq; auto. apply (LEM B HB). }
+          ++  apply associativity1. apply exchange2. apply exchange1. apply weakening.
+              **  destruct HB as [HB | HB].
+                  { apply (one_var_free_lemma _ _ _ Ht HB). }
+                  { rewrite closed_subst_eq; apply HB. }
+              **  destruct X,X1. destruct HC as [HC | HC].
+                  { apply (H (num_conn C) HC' C (eq_refl (num_conn C)) n0 s t H1 HC). }
+                  { rewrite closed_subst_eq, closed_subst_eq; auto. apply (LEM C HC). }
+      --  unfold num_conn. fold num_conn. apply ord_lt_succ. 
+          rewrite <- plus_n_Sm. rewrite <- ord_succ_nat. rewrite plus_n_Sm. rewrite <- plus_assoc.
+          rewrite (plus_comm (S _)). rewrite <- plus_n_Sm. rewrite <- plus_n_Sm. rewrite <- ord_succ_nat. repeat rewrite ord_max_succ_succ.
+          apply ord_lt_succ. apply ord_lt_succ. rewrite ord_max_nat. apply nat_ord_lt. lia.
+      --  apply ord_succ_nf. apply nf_nat.
 - apply exchange1. inversion H0.
   unfold substitution. fold substitution. pose proof (univ_free_var _ _ _ H2) as Heq. rewrite Heq.
-  apply (ord_incr _ _ (w_tower ((num_conn (univ m B))+(num_conn (univ m B))))).
-  + apply w_rule2. intros k. apply exchange1. apply (ord_incr _ _ (ord_succ ( ord_succ (w_tower ((num_conn B)+(num_conn B)))))).
-    * apply (quantification2 _ _ _ (represent k)).
-      { apply repr_closed. }
-      { destruct (correct_closed_t _ _ H1) as [Hs Ht].
-        rewrite (substitution_order B m n0 s _ Hs (repr_closed k) Heq).
-        rewrite (substitution_order B m n0 t _ Ht (repr_closed k) Heq).
-        rewrite <- (num_conn_sub B m (represent k)).
-        apply (H n (leq_refl n) (substitution B m (represent k))); auto.
-        { rewrite num_conn_sub. auto. }
-        { apply free_list_univ_sub; auto. apply repr_closed. }
-        }
-    * unfold num_conn. fold num_conn. fold w_tower. rewrite <- plus_n_Sm. apply w_tower_succ2.
-    * apply w_tower_nf.
-  + apply ord_succ_monot.
-  + apply ord_succ_nf. apply w_tower_nf.
+  unfold num_conn. fold num_conn. rewrite <- plus_n_Sm. rewrite plus_comm. rewrite <- plus_n_Sm. repeat rewrite <- ord_succ_nat.
+  apply w_rule2. intros k. apply exchange1. apply (quantification2 _ _ _ (represent k)). apply repr_closed.
+  destruct (correct_closed_t _ _ H1) as [Hs Ht].
+  rewrite (substitution_order B m n0 s _ Hs (repr_closed k) Heq).
+  rewrite (substitution_order B m n0 t _ Ht (repr_closed k) Heq).
+  rewrite <- (num_conn_sub B m (represent k)).
+  apply (H n (leq_refl n) (substitution B m (represent k))); auto.
+  + rewrite num_conn_sub. auto.
+  + apply free_list_univ_sub; auto. apply repr_closed.
 Qed.
 
 Lemma Q3_lemma : forall n, Q3 n.
@@ -743,7 +778,7 @@ Lemma LEM_term : forall (A : formula) (n : nat) (s t : term),
   correct_a (equ s t) = true ->
   free_list A = [n] ->
   PA_omega_theorem (lor (neg (substitution A n s)) (substitution A n t))
-                   0 (ord_succ (w_tower ((num_conn A)+(num_conn A)))).
+                   0 (ord_succ (nat_ord ((num_conn A)+(num_conn A)))).
 Proof. apply Q1_lemma. Qed.
 
 (*
