theories/Logic/Peano.v
@@ -20,14 +20,14 @@ Notation "A1 ~> A2" := (impl A1 A2) (at level 60).
 Notation "t # s" := (atom (equ t s)) (at level 80).
 
 Inductive Peano_Theorems_Base : formula -> nat -> ord -> Type :=
-| FOL1 : forall (A B : formula), Peano_Theorems_Base (A ~> (B ~> A)) 0 (ord_succ (ord_succ (w_tower (num_conn A + num_conn A))))
-| FOL2 : forall (A B C : formula), Peano_Theorems_Base ((A ~> (B ~> C)) ~> ((A ~> B) ~> (A ~> C))) (num_conn (neg B)) (ord_succ (ord_max (ord_succ (w_tower (num_conn (lor (neg A) B) + num_conn (lor (neg A) B)))) ((ord_succ (w_tower (num_conn (lor (neg A) (lor (neg B) C)) + num_conn (lor (neg A) (lor (neg B) C))))))))
-| FOL3 : forall (A B : formula), Peano_Theorems_Base ((neg A ~> neg B) ~> ((neg A ~> B) ~> A)) 0 (ord_succ (ord_max (ord_succ (ord_succ (ord_succ (w_tower (num_conn (A) + num_conn (A)))))) ((ord_succ (ord_max (ord_succ (ord_succ (ord_succ (w_tower (num_conn A + num_conn A))))) (ord_succ (ord_succ (w_tower (num_conn (neg B) + num_conn (neg B))))))))))
-| FOL4 : forall (A : formula) (n : nat) (t : term), closed_t t = true -> Peano_Theorems_Base (lor (neg(univ n A)) (substitution A n t)) 0 (ord_succ (ord_succ (w_tower (num_conn (substitution A n t) + num_conn (substitution A n t)))))
-| FOL5 : forall (A B : formula) (n : nat), member n (free_list A) = false -> Peano_Theorems_Base ((univ n (A ~> B)) ~> (A ~> (univ n B))) 0 (cons (ord_succ (ord_succ (w_tower (num_conn (lor (neg A) B) + num_conn (lor (neg A) B))))) 0 Zero)
+| FOL1 : forall (A B : formula), Peano_Theorems_Base (A ~> (B ~> A)) 0 (ord_succ (ord_succ (nat_ord (num_conn A + num_conn A))))
+| FOL2 : forall (A B C : formula), Peano_Theorems_Base ((A ~> (B ~> C)) ~> ((A ~> B) ~> (A ~> C))) (num_conn (neg B)) (ord_succ (ord_max (ord_succ (nat_ord (num_conn (lor (neg A) B) + num_conn (lor (neg A) B)))) ((ord_succ (nat_ord (num_conn (lor (neg A) (lor (neg B) C)) + num_conn (lor (neg A) (lor (neg B) C))))))))
+| FOL3 : forall (A B : formula), Peano_Theorems_Base ((neg A ~> neg B) ~> ((neg A ~> B) ~> A)) 0 (ord_succ (ord_max (ord_succ (ord_succ (ord_succ (nat_ord (num_conn (A) + num_conn (A)))))) ((ord_succ (ord_max (ord_succ (ord_succ (ord_succ (nat_ord (num_conn A + num_conn A))))) (ord_succ (ord_succ (nat_ord (num_conn (neg B) + num_conn (neg B))))))))))
+| FOL4 : forall (A : formula) (n : nat) (t : term), closed_t t = true -> Peano_Theorems_Base (lor (neg(univ n A)) (substitution A n t)) 0 (ord_succ (ord_succ (nat_ord (num_conn (substitution A n t) + num_conn (substitution A n t)))))
+| FOL5 : forall (A B : formula) (n : nat), member n (free_list A) = false -> Peano_Theorems_Base ((univ n (A ~> B)) ~> (A ~> (univ n B))) 0 (ord_succ (ord_succ (ord_succ (nat_ord (num_conn (lor (neg A) B) + num_conn (lor (neg A) B))))))
 | MP : forall (A B : formula) (n m : nat) (alpha beta : ord), Peano_Theorems_Base (A ~> B) n alpha -> Peano_Theorems_Base A m beta -> Peano_Theorems_Base B (max (max m n) (num_conn (neg A))) (ord_succ (ord_max beta alpha))
-| UG : forall (A : formula) (n m : nat) (alpha : ord), Peano_Theorems_Base A m alpha -> Peano_Theorems_Base (univ n A) m (cons alpha 0 Zero) 
-| equ_trans : forall (t s r : term), Peano_Theorems_Base  ((t # s) ~> ((s # r) ~> (t # r))) 0 (ord_succ (ord_succ (w_tower (num_conn (atom (equ s t))))))
+| UG : forall (A : formula) (n m : nat) (alpha : ord), Peano_Theorems_Base A m alpha -> Peano_Theorems_Base (univ n A) m (ord_succ alpha) 
+| equ_trans : forall (t s r : term), Peano_Theorems_Base  ((t # s) ~> ((s # r) ~> (t # r))) 0 (ord_succ (ord_succ (nat_ord (num_conn (atom (equ s t))))))
 | equ_succ : forall (t s : term),  Peano_Theorems_Base ((t # s) ~> ((succ t) # (succ s))) 0 (ord_succ Zero)
 | non_zero : forall (t : term), Peano_Theorems_Base (neg (zero # (succ t))) 0 Zero
 | succ_equ : forall (t s : term),  Peano_Theorems_Base ((succ t # succ s) ~> (t # s)) 0 (ord_succ Zero)
@@ -35,17 +35,17 @@ Inductive Peano_Theorems_Base : formula -> nat -> ord -> Type :=
 | plS : forall (t s : term), Peano_Theorems_Base ((plus t (succ s)) # (succ (plus t s))) 0 Zero
 | ml0 : forall (t : term), Peano_Theorems_Base ((times t zero) # zero) 0 Zero
 | mlS : forall (t s : term), Peano_Theorems_Base ((times t (succ s)) # (plus (times t s) t)) 0 Zero
-| induct : forall (A : formula) (n : nat), Peano_Theorems_Base (substitution A n zero ~> ((univ n (A ~> (substitution A n (succ (var n))))) ~> (univ n A))) 0 (cons (w_tower (S (S (S (num_conn A + num_conn A))))) 0 Zero).
+| induct : forall (A : formula) (n : nat), Peano_Theorems_Base (substitution A n zero ~> ((univ n (A ~> (substitution A n (succ (var n))))) ~> (univ n A))) 0 (ord_succ (cons (nat_ord 1) 1 Zero)).
 
 Inductive Peano_Theorems_Implication : formula -> nat -> ord -> Type :=
-| I_FOL1 : forall (A B : formula), Peano_Theorems_Implication (A ~> (B ~> A)) 0 (ord_succ (ord_succ (w_tower (num_conn A + num_conn A))))
-| I_FOL2 : forall (A B C : formula), Peano_Theorems_Implication ((A ~> (B ~> C)) ~> ((A ~> B) ~> (A ~> C))) (num_conn (neg B)) (ord_succ (ord_max (ord_succ (w_tower (num_conn (lor (neg A) B) + num_conn (lor (neg A) B)))) ((ord_succ (w_tower (num_conn (lor (neg A) (lor (neg B) C)) + num_conn (lor (neg A) (lor (neg B) C))))))))
-| I_FOL3 : forall (A B : formula), Peano_Theorems_Implication ((neg A ~> neg B) ~> ((neg A ~> B) ~> A)) 0 (ord_succ (ord_max (ord_succ (ord_succ (ord_succ (w_tower (num_conn (A) + num_conn (A)))))) ((ord_succ (ord_max (ord_succ (ord_succ (ord_succ (w_tower (num_conn A + num_conn A))))) (ord_succ (ord_succ (w_tower (num_conn (neg B) + num_conn (neg B))))))))))
-| I_FOL4 : forall (A : formula) (n : nat) (t : term), closed_t t = true -> Peano_Theorems_Implication (lor (neg(univ n A)) (substitution A n t)) 0 (ord_succ (ord_succ (w_tower (num_conn (substitution A n t) + num_conn (substitution A n t)))))
-| I_FOL5 : forall (A B : formula) (n : nat), member n (free_list A) = false -> Peano_Theorems_Implication ((univ n (A ~> B)) ~> (A ~> (univ n B))) 0 (cons (ord_succ (ord_succ (w_tower (num_conn (lor (neg A) B) + num_conn (lor (neg A) B))))) 0 Zero)
+| I_FOL1 : forall (A B : formula), Peano_Theorems_Implication (A ~> (B ~> A)) 0 (ord_succ (ord_succ (nat_ord (num_conn A + num_conn A))))
+| I_FOL2 : forall (A B C : formula), Peano_Theorems_Implication ((A ~> (B ~> C)) ~> ((A ~> B) ~> (A ~> C))) (num_conn (neg B)) (ord_succ (ord_max (ord_succ (nat_ord (num_conn (lor (neg A) B) + num_conn (lor (neg A) B)))) ((ord_succ (nat_ord (num_conn (lor (neg A) (lor (neg B) C)) + num_conn (lor (neg A) (lor (neg B) C))))))))
+| I_FOL3 : forall (A B : formula), Peano_Theorems_Implication ((neg A ~> neg B) ~> ((neg A ~> B) ~> A)) 0 (ord_succ (ord_max (ord_succ (ord_succ (ord_succ (nat_ord (num_conn (A) + num_conn (A)))))) ((ord_succ (ord_max (ord_succ (ord_succ (ord_succ (nat_ord (num_conn A + num_conn A))))) (ord_succ (ord_succ (nat_ord (num_conn (neg B) + num_conn (neg B))))))))))
+| I_FOL4 : forall (A : formula) (n : nat) (t : term), closed_t t = true -> Peano_Theorems_Implication (lor (neg(univ n A)) (substitution A n t)) 0 (ord_succ (ord_succ (nat_ord (num_conn (substitution A n t) + num_conn (substitution A n t)))))
+| I_FOL5 : forall (A B : formula) (n : nat), member n (free_list A) = false -> Peano_Theorems_Implication ((univ n (A ~> B)) ~> (A ~> (univ n B))) 0 (ord_succ (ord_succ (ord_succ (nat_ord (num_conn (lor (neg A) B) + num_conn (lor (neg A) B))))))
 | I_MP : forall (A B : formula) (n m : nat) (alpha beta : ord), Peano_Theorems_Implication (A ~> B) n alpha -> Peano_Theorems_Implication A m beta -> Peano_Theorems_Implication B (max (max m n) (num_conn (neg A))) (ord_succ (ord_max beta alpha))
-| I_UG : forall (A : formula) (n m : nat) (alpha : ord), Peano_Theorems_Implication A m alpha -> (forall t, closed_t t = true -> Peano_Theorems_Implication (substitution A n t) m alpha) -> Peano_Theorems_Implication (univ n A) m (cons alpha 0 Zero) 
-| I_equ_trans : forall (t s r : term), Peano_Theorems_Implication  ((t # s) ~> ((s # r) ~> (t # r))) 0 (ord_succ (ord_succ (w_tower (num_conn (atom (equ s t))))))
+| I_UG : forall (A : formula) (n m : nat) (alpha : ord), Peano_Theorems_Implication A m alpha -> (forall t, closed_t t = true -> Peano_Theorems_Implication (substitution A n t) m alpha) -> Peano_Theorems_Implication (univ n A) m (ord_succ alpha) 
+| I_equ_trans : forall (t s r : term), Peano_Theorems_Implication  ((t # s) ~> ((s # r) ~> (t # r))) 0 (ord_succ (ord_succ (nat_ord (num_conn (atom (equ s t))))))
 | I_equ_succ : forall (t s : term),  Peano_Theorems_Implication ((t # s) ~> ((succ t) # (succ s))) 0 (ord_succ Zero)
 | I_non_zero : forall (t : term), Peano_Theorems_Implication (neg (zero # (succ t))) 0 Zero
 | I_succ_equ : forall (t s : term),  Peano_Theorems_Implication ((succ t # succ s) ~> (t # s)) 0 (ord_succ Zero)
@@ -53,7 +53,7 @@ Inductive Peano_Theorems_Implication : formula -> nat -> ord -> Type :=
 | I_plS : forall (t s : term), Peano_Theorems_Implication ((plus t (succ s)) # (succ (plus t s))) 0 Zero
 | I_ml0 : forall (t : term), Peano_Theorems_Implication ((times t zero) # zero) 0 Zero
 | I_mlS : forall (t s : term), Peano_Theorems_Implication ((times t (succ s)) # (plus (times t s) t)) 0 Zero
-| I_induct : forall (A : formula) (n : nat), Peano_Theorems_Implication (substitution A n zero ~> ((univ n (A ~> (substitution A n (succ (var n))))) ~> (univ n A))) 0 (cons (w_tower (S (S (S (num_conn A + num_conn A))))) 0 Zero).
+| I_induct : forall (A : formula) (n : nat), Peano_Theorems_Implication (substitution A n zero ~> ((univ n (A ~> (substitution A n (succ (var n))))) ~> (univ n A))) 0 (ord_succ (cons (nat_ord 1) 1 Zero)).
 
 Fixpoint inductive_chain (A : formula) (n m : nat) : formula :=
 match m with
@@ -81,55 +81,51 @@ intros. induction m.
 - simpl. rewrite IHm. repeat rewrite closed_subst_eq; auto. rewrite H. auto.
 Qed.
 
-Lemma inductive_implication_theorem_aux : forall A n m, free_list A = [n] -> PA_omega_theorem (inductive_implication A n m) 0 (ord_add (w_tower (S (num_conn A + num_conn A))) (nat_ord (3 * (S m)))).
+Lemma inductive_implication_theorem_aux : forall A n m, free_list A = [n] -> PA_omega_theorem (inductive_implication A n m) 0 (ord_add (nat_ord (S (num_conn A + num_conn A))) (nat_ord (3 * (S m)))).
 intros. induction m.
-- apply (ord_incr _ _ (ord_succ (w_tower (num_conn A + num_conn A)))).
+- apply (ord_incr _ _ (ord_succ (nat_ord (num_conn A + num_conn A)))).
   + apply exchange1. assert (num_conn A = num_conn (substitution A n zero)). rewrite num_conn_sub. auto. rewrite H0. apply LEM. rewrite closed_univ_sub; auto. simpl. case (closed A); auto. rewrite H. rewrite eq_nat_refl. auto.
-  + apply (lt_trans _ _ _ (w_tower_succ _)). apply add_right_incr_corr. simpl. apply zero_lt.
-  + apply nf_add. apply w_tower_nf. apply nf_nat.
-- assert ((ord_add (w_tower (S (num_conn A + num_conn A))) (nat_ord (3 * S (S m)))) = (ord_succ (ord_max (ord_succ (ord_succ (ord_add (w_tower (S (num_conn A + num_conn A))) (nat_ord (3 * (S m)))))) (ord_succ (ord_succ (w_tower (num_conn A + num_conn A))))))).
-  { simpl. assert (ord_ltb Zero (w_tower (num_conn A + num_conn A)) = true). destruct (num_conn A); auto. rewrite (ltb_asymm _ _ H0). rewrite (ord_lt_ne _ _ H0). assert ((ord_max (ord_succ (ord_succ (cons (w_tower (num_conn A + num_conn A)) 0 (cons Zero (m + S (m + S (m + 0))) Zero)))) (ord_succ (ord_succ (w_tower (num_conn A + num_conn A))))) = (ord_succ (ord_succ (cons (w_tower (num_conn A + num_conn A)) 0 (cons Zero (m + S (m + S (m + 0))) Zero))))).
-    apply ord_max_lem2. apply ltb_asymm. apply ord_lt_ltb. apply ord_lt_succ. apply ord_lt_succ. apply ord_lt_self. rewrite H1. simpl. case (w_tower (num_conn A + num_conn A)) eqn:X. destruct (num_conn A); inversion X. simpl. repeat rewrite plus_n_Sm. auto. }
-  rewrite H0.
-  + destruct m.
-    * unfold inductive_implication. unfold inductive_chain. unfold "~>". apply associativity2. assert (max 0 0 = 0). lia. destruct H1. apply demorgan2. 
-      --  apply negation2. apply associativity1. apply exchange3. apply associativity2. apply weakening. apply closed_univ_sub_repr. simpl. rewrite H. rewrite eq_nat_refl. destruct (closed A); auto. auto.
-      --  apply associativity1. apply exchange1. apply weakening. apply closed_univ_sub; auto. simpl. rewrite H. rewrite eq_nat_refl. destruct (closed A); auto. simpl. assert (num_conn A = num_conn (substitution A n (succ zero))). rewrite num_conn_sub. auto. rewrite H1. apply LEM. rewrite closed_univ_sub; simpl; auto. rewrite H. rewrite eq_nat_refl. destruct (closed A); auto. 
-    * unfold inductive_implication in *. unfold inductive_chain. fold inductive_chain. unfold "~>". apply exchange4. apply exchange2. apply exchange1. assert (max 0 0 = 0). lia. destruct H1. apply demorgan2.
-      --  apply negation2. apply exchange1. apply exchange2. apply exchange4. apply exchange2. apply exchange1. apply weakening. apply closed_univ_sub_repr. simpl. rewrite H. rewrite eq_nat_refl. destruct (closed A); auto. auto. 
-      --  apply exchange1. apply exchange4. apply exchange2. apply associativity2. apply weakening. simpl. rewrite ind_imp_closed; auto. apply closed_univ_sub; auto. simpl. rewrite H. rewrite eq_nat_refl. destruct (closed A); auto. simpl. assert (num_conn A = num_conn (substitution A n (succ (succ (represent m))))). rewrite num_conn_sub. auto. rewrite H1. apply LEM. rewrite closed_univ_sub; simpl; auto. rewrite H. rewrite eq_nat_refl. destruct (closed A); auto. apply repr_closed.
+  + rewrite <- ord_add_nat. rewrite ord_succ_nat. apply nat_ord_lt. lia.
+  + apply nf_add; apply nf_nat.
+- assert ((ord_add (nat_ord (S (num_conn A + num_conn A))) (nat_ord (3 * S (S m)))) = (ord_succ (ord_max (ord_succ (ord_succ (ord_add (nat_ord (S (num_conn A + num_conn A))) (nat_ord (3 * (S m)))))) (ord_succ (ord_succ (nat_ord (num_conn A + num_conn A))))))).
+  { repeat rewrite <- ord_add_nat. repeat rewrite ord_max_succ_succ. rewrite ord_max_lem2. repeat rewrite ord_succ_nat. unfold mul. simpl. rewrite plus_n_0. repeat rewrite plus_n_Sm. auto. apply ltb_asymm. apply ord_lt_ltb. apply nat_ord_lt. lia. }
+  rewrite H0. destruct m.
+  + unfold inductive_implication. unfold inductive_chain. unfold "~>". apply associativity2. assert (max 0 0 = 0). lia. destruct H1. apply demorgan2. 
+    *  apply negation2. apply associativity1. apply exchange3. apply associativity2. apply weakening. apply closed_univ_sub_repr. simpl. rewrite H. rewrite eq_nat_refl. destruct (closed A); auto. auto.
+    *  apply associativity1. apply exchange1. apply weakening. apply closed_univ_sub; auto. simpl. rewrite H. rewrite eq_nat_refl. destruct (closed A); auto. simpl. assert (num_conn A = num_conn (substitution A n (succ zero))). rewrite num_conn_sub. auto. rewrite H1. apply LEM. rewrite closed_univ_sub; simpl; auto. rewrite H. rewrite eq_nat_refl. destruct (closed A); auto. 
+  + unfold inductive_implication in *. unfold inductive_chain. fold inductive_chain. unfold "~>". apply exchange4. apply exchange2. apply exchange1. assert (max 0 0 = 0). lia. destruct H1. apply demorgan2.
+    * apply negation2. apply exchange1. apply exchange2. apply exchange4. apply exchange2. apply exchange1. apply weakening. apply closed_univ_sub_repr. simpl. rewrite H. rewrite eq_nat_refl. destruct (closed A); auto. auto. 
+    * apply exchange1. apply exchange4. apply exchange2. apply associativity2. apply weakening. simpl. rewrite ind_imp_closed; auto. apply closed_univ_sub; auto. simpl. rewrite H. rewrite eq_nat_refl. destruct (closed A); auto. simpl. assert (num_conn A = num_conn (substitution A n (succ (succ (represent m))))). rewrite num_conn_sub. auto. rewrite H1. apply LEM. rewrite closed_univ_sub; simpl; auto. rewrite H. rewrite eq_nat_refl. destruct (closed A); auto. apply repr_closed.
 Qed.
 
-Lemma inductive_implication_theorem_aux' : forall A n m, closed A = true -> PA_omega_theorem (inductive_implication A n m) 0 (ord_add (w_tower (S (num_conn A + num_conn A))) (nat_ord (3 * (S m)))).
+Lemma inductive_implication_theorem_aux' : forall A n m, closed A = true -> PA_omega_theorem (inductive_implication A n m) 0 (ord_add (nat_ord (S (num_conn A + num_conn A))) (nat_ord (3 * (S m)))).
 intros. induction m.
-- apply (ord_incr _ _ (ord_succ (w_tower (num_conn A + num_conn A)))).
+- apply (ord_incr _ _ (ord_succ (nat_ord (num_conn A + num_conn A)))).
   + apply exchange1. assert (num_conn A = num_conn (substitution A n zero)). rewrite num_conn_sub. auto. rewrite H0. apply LEM. rewrite closed_univ_sub; auto. simpl. rewrite H. auto.
-  + apply (lt_trans _ _ _ (w_tower_succ _)). apply add_right_incr_corr. simpl. apply zero_lt.
-  + apply nf_add. apply w_tower_nf. apply nf_nat.
-- assert ((ord_add (w_tower (S (num_conn A + num_conn A))) (nat_ord (3 * S (S m)))) = (ord_succ (ord_max (ord_succ (ord_succ (ord_add (w_tower (S (num_conn A + num_conn A))) (nat_ord (3 * (S m)))))) (ord_succ (ord_succ (w_tower (num_conn A + num_conn A))))))).
-  { simpl. assert (ord_ltb Zero (w_tower (num_conn A + num_conn A)) = true). destruct (num_conn A); auto. rewrite (ltb_asymm _ _ H0). rewrite (ord_lt_ne _ _ H0). assert ((ord_max (ord_succ (ord_succ (cons (w_tower (num_conn A + num_conn A)) 0 (cons Zero (m + S (m + S (m + 0))) Zero)))) (ord_succ (ord_succ (w_tower (num_conn A + num_conn A))))) = (ord_succ (ord_succ (cons (w_tower (num_conn A + num_conn A)) 0 (cons Zero (m + S (m + S (m + 0))) Zero))))).
-    apply ord_max_lem2. apply ltb_asymm. apply ord_lt_ltb. apply ord_lt_succ. apply ord_lt_succ. apply ord_lt_self. rewrite H1. simpl. case (w_tower (num_conn A + num_conn A)) eqn:X. destruct (num_conn A); inversion X. simpl. repeat rewrite plus_n_Sm. auto. }
-  rewrite H0.
-  + destruct m.
-    * unfold inductive_implication. unfold inductive_chain. unfold "~>". apply associativity2. assert (max 0 0 = 0). lia. destruct H1. apply demorgan2. 
-      --  apply negation2. apply associativity1. apply exchange3. apply associativity2. apply weakening. apply closed_univ_sub_repr. simpl. rewrite H. auto. auto.
-      --  apply associativity1. apply exchange1. apply weakening. apply closed_univ_sub; auto. simpl. rewrite H. auto. simpl. assert (num_conn A = num_conn (substitution A n (succ zero))). rewrite num_conn_sub. auto. rewrite H1. apply LEM. rewrite closed_univ_sub; simpl; auto. rewrite H. auto. 
-    * unfold inductive_implication in *. unfold inductive_chain. fold inductive_chain. unfold "~>". apply exchange4. apply exchange2. apply exchange1. assert (max 0 0 = 0). lia. destruct H1. apply demorgan2.
-      --  apply negation2. apply exchange1. apply exchange2. apply exchange4. apply exchange2. apply exchange1. apply weakening. apply closed_univ_sub_repr. simpl. rewrite H. auto. auto. 
-      --  apply exchange1. apply exchange4. apply exchange2. apply associativity2. apply weakening. simpl. rewrite ind_imp_closed'; auto. apply closed_univ_sub; auto. simpl. rewrite H. auto. simpl. assert (num_conn A = num_conn (substitution A n (succ (succ (represent m))))). rewrite num_conn_sub. auto. rewrite H1. apply LEM. rewrite closed_univ_sub; simpl; auto. rewrite H. auto. apply repr_closed.
+  + rewrite <- ord_succ_nat. apply add_right_incr_corr. apply zero_lt.
+  + apply nf_add; apply nf_nat.
+- assert ((ord_add (nat_ord (S (num_conn A + num_conn A))) (nat_ord (3 * S (S m)))) = (ord_succ (ord_max (ord_succ (ord_succ (ord_add (nat_ord (S (num_conn A + num_conn A))) (nat_ord (3 * (S m)))))) (ord_succ (ord_succ (nat_ord (num_conn A + num_conn A))))))).
+  { repeat rewrite <- ord_add_nat. repeat rewrite ord_max_succ_succ. rewrite ord_max_lem2. repeat rewrite ord_succ_nat. unfold mul. simpl. rewrite plus_n_0. repeat rewrite plus_n_Sm. auto. apply ltb_asymm. apply ord_lt_ltb. apply nat_ord_lt. lia. }
+  rewrite H0. destruct m.
+  + unfold inductive_implication. unfold inductive_chain. unfold "~>". apply associativity2. assert (max 0 0 = 0). lia. destruct H1. apply demorgan2. 
+    * apply negation2. apply associativity1. apply exchange3. apply associativity2. apply weakening. apply closed_univ_sub_repr. simpl. rewrite H. auto. auto.
+    * apply associativity1. apply exchange1. apply weakening. apply closed_univ_sub; auto. simpl. rewrite H. auto. simpl. assert (num_conn A = num_conn (substitution A n (succ zero))). rewrite num_conn_sub. auto. rewrite H1. apply LEM. rewrite closed_univ_sub; simpl; auto. rewrite H. auto. 
+  + unfold inductive_implication in *. unfold inductive_chain. fold inductive_chain. unfold "~>". apply exchange4. apply exchange2. apply exchange1. assert (max 0 0 = 0). lia. destruct H1. apply demorgan2.
+    * apply negation2. apply exchange1. apply exchange2. apply exchange4. apply exchange2. apply exchange1. apply weakening. apply closed_univ_sub_repr. simpl. rewrite H. auto. auto. 
+    * apply exchange1. apply exchange4. apply exchange2. apply associativity2. apply weakening. simpl. rewrite ind_imp_closed'; auto. apply closed_univ_sub; auto. simpl. rewrite H. auto. simpl. assert (num_conn A = num_conn (substitution A n (succ (succ (represent m))))). rewrite num_conn_sub. auto. rewrite H1. apply LEM. rewrite closed_univ_sub; simpl; auto. rewrite H. auto. apply repr_closed.
 Qed.
 
-Lemma inductive_implication_theorem : forall A n m, free_list A = [n] -> PA_omega_theorem (inductive_implication A n m) 0 (w_tower (S (S (num_conn A + num_conn A)))).
-intros. refine (ord_incr _ _ (ord_add (w_tower (S (num_conn A + num_conn A))) (nat_ord (3 * (S m)))) _ _ _ (w_tower_nf _)). apply inductive_implication_theorem_aux. auto.
-simpl. assert (ord_ltb Zero (w_tower (num_conn A + num_conn A)) = true). destruct (num_conn A); auto. rewrite (ltb_asymm _ _ H0). rewrite (ord_lt_ne _ _ H0). apply head_lt. apply ord_lt_self. 
+Lemma inductive_implication_theorem : forall A n m, free_list A = [n] -> PA_omega_theorem (inductive_implication A n m) 0 (cons (nat_ord 1) 0 Zero).
+intros. refine (ord_incr _ _ (ord_add (nat_ord (S (num_conn A + num_conn A))) (nat_ord (3 * (S m)))) _ _ _ (single_nf _ _ (nf_nat _))). apply inductive_implication_theorem_aux. auto.
+repeat rewrite <- ord_add_nat. apply nat_lt_omega. apply zero_lt.
 Qed.
 
-Lemma inductive_implication_theorem' : forall A n m, closed A = true -> PA_omega_theorem (inductive_implication A n m) 0 (w_tower (S (S (num_conn A + num_conn A)))).
-intros. refine (ord_incr _ _ (ord_add (w_tower (S (num_conn A + num_conn A))) (nat_ord (3 * (S m)))) _ _ _ (w_tower_nf _)). apply inductive_implication_theorem_aux'. auto.
-simpl. assert (ord_ltb Zero (w_tower (num_conn A + num_conn A)) = true). destruct (num_conn A); auto. rewrite (ltb_asymm _ _ H0). rewrite (ord_lt_ne _ _ H0). apply head_lt. apply ord_lt_self. 
+Lemma inductive_implication_theorem' : forall A n m, closed A = true -> PA_omega_theorem (inductive_implication A n m) 0 (cons (nat_ord 1) 0 Zero).
+intros. refine (ord_incr _ _ (ord_add (nat_ord (S (num_conn A + num_conn A))) (nat_ord (3 * (S m)))) _ _ _ (single_nf _ _ (nf_nat _))). apply inductive_implication_theorem_aux'. auto.
+repeat rewrite <- ord_add_nat. apply nat_lt_omega. apply zero_lt.
 Qed.
 
-Lemma induction_iterate : forall (A : formula) (n m : nat) (t : term), PA_omega_theorem (lor (lor (lor (inductive_chain A n (S m)) (substitution A n t)) (neg (substitution A n zero))) (neg (univ n (lor (neg A) (substitution A n (succ (var n))))))) 0 (w_tower (S (S (num_conn A + num_conn A)))) -> PA_omega_theorem (lor (lor (lor (inductive_chain A n m) (substitution A n t)) (neg (substitution A n zero))) (neg (univ n (lor (neg A) (substitution A n (succ (var n))))))) 0 (ord_succ (w_tower (S (S (num_conn A + num_conn A))))).
+Lemma induction_iterate : forall (A : formula) (n m : nat) (t : term), PA_omega_theorem (lor (lor (lor (inductive_chain A n (S m)) (substitution A n t)) (neg (substitution A n zero))) (neg (univ n (lor (neg A) (substitution A n (succ (var n))))))) 0 (nat_ord (S (S (num_conn A + num_conn A)))) -> PA_omega_theorem (lor (lor (lor (inductive_chain A n m) (substitution A n t)) (neg (substitution A n zero))) (neg (univ n (lor (neg A) (substitution A n (succ (var n))))))) 0 (ord_succ (nat_ord (S (S (num_conn A + num_conn A))))).
 Proof.
 intros. apply exchange1. apply contraction2. apply associativity2. apply (quantification2 _ _ _ (represent (S m))). apply repr_closed. unfold inductive_chain in H. fold inductive_chain in H. unfold "~>" in H.
 simpl in H. simpl. repeat apply associativity1. apply exchange1. apply associativity1. apply associativity1. apply exchange4. apply associativity2. apply exchange3. apply associativity1. apply exchange4. apply associativity2. apply exchange2.
@@ -150,35 +146,40 @@ intros A n m. induction m; intros.
 - pose proof (IHm _ _ (induction_iterate_general _ _ _ _ _ H)). rewrite ord_add_succ_nat_succ_add. auto. apply (ord_nf _ _ _ H).
 Qed.
 
-Lemma induction_final : forall (A : formula) (n m : nat) (t : term) (alpha : ord), PA_omega_theorem (lor (lor (lor (inductive_chain A n (S m)) (substitution A n t)) (neg (substitution A n zero))) (neg (univ n (lor (neg A) (substitution A n (succ (var n))))))) 0 alpha -> PA_omega_theorem (lor (lor (substitution A n t) (neg (substitution A n zero))) (neg (univ n (lor (neg A) (substitution A n (succ (var n))))))) 0 (ord_succ (ord_add alpha (nat_ord (S m)))).
+Lemma induction_final : forall (A : formula) (n m : nat) (t : term) (alpha : ord),
+    PA_omega_theorem (lor (lor (lor (inductive_chain A n (S m)) (substitution A n t)) (neg (substitution A n zero))) (neg (univ n (lor (neg A) (substitution A n (succ (var n))))))) 0 alpha ->
+        PA_omega_theorem (lor (lor (substitution A n t) (neg (substitution A n zero))) (neg (univ n (lor (neg A) (substitution A n (succ (var n))))))) 0 (ord_succ (ord_add alpha (nat_ord (S m)))).
 Proof.
 intros. pose proof (induction_terminate _ _ _ _ _ H). unfold inductive_chain in H0. unfold "~>" in H0. apply exchange1. apply contraction2. apply associativity2. apply (quantification2 _ _ _ (represent 0)). apply repr_closed. simpl.
 rewrite sub_succ_self. apply associativity1. apply associativity1. apply exchange4. apply exchange2. auto.
 Qed.
 
-Lemma induction_aux : forall A n m, free_list A = [n] -> PA_omega_theorem (lor (lor (substitution A n (represent m)) (neg (substitution A n zero))) (neg (univ n (lor (neg A) (substitution A n (succ (var n))))))) 0 (w_tower (S (S (S (num_conn A + num_conn A))))).
+Lemma induction_aux : forall A n m, free_list A = [n] -> PA_omega_theorem (lor (lor (substitution A n (represent m)) (neg (substitution A n zero))) (neg (univ n (lor (neg A) (substitution A n (succ (var n))))))) 0 (cons (nat_ord 1) 1 Zero).
 Proof.
-intros. pose proof (inductive_implication_theorem _ _  m H). apply (ord_incr _ _  (ord_succ (ord_add (ord_succ (ord_succ (w_tower (S (S (num_conn A + num_conn A)))))) (nat_ord (S m))))).
-- destruct m.
-  + apply exchange1. apply weakening; auto. simpl. case (closed A) eqn:X; auto.
+intros. pose proof (inductive_implication_theorem _ _  m H). destruct m.
+- apply (ord_incr _ _  (ord_succ (ord_add (ord_succ (ord_succ (nat_ord (S (S (num_conn A + num_conn A)))))) (nat_ord (S 0))))).
+  +  apply exchange1. apply weakening; auto. simpl. case (closed A) eqn:X; auto.
     * rewrite closed_free_list in H; auto. inversion H.
     * simpl. rewrite H. rewrite (free_list_sub_self_eq _ _ (var n)); auto. simpl. rewrite eq_nat_refl. auto.
-    * apply exchange1. apply (ord_incr _ _ (ord_succ (w_tower (num_conn A + num_conn A)))). rewrite <- (num_conn_sub _ n zero). apply LEM. apply closed_univ_sub. simpl. rewrite H. rewrite eq_nat_refl. destruct (closed A); auto. auto. rewrite ord_add_one_succ. apply ord_lt_succ. simpl. apply (lt_trans _ _ _ (omega_exp_incr _)). apply head_lt. apply ord_lt_self. repeat apply ord_succ_nf. apply w_tower_nf. apply nf_add. repeat apply ord_succ_nf. apply w_tower_nf. apply nf_nat. 
-  + unfold inductive_implication in H0. unfold represent in H0. fold represent in H0. apply induction_final. auto. unfold inductive_chain. fold inductive_chain. apply associativity2. apply associativity2. apply associativity2. apply exchange3. apply associativity1. apply exchange4. apply associativity2. apply exchange3. apply weakening.
+    * apply exchange1. apply (ord_incr _ _ (ord_succ (nat_ord (num_conn A + num_conn A)))). rewrite <- (num_conn_sub _ n zero). apply LEM. apply closed_univ_sub. simpl. rewrite H. rewrite eq_nat_refl. destruct (closed A); auto. auto. rewrite ord_add_one_succ. repeat rewrite ord_succ_nat. apply nat_ord_lt. lia. repeat apply ord_succ_nf. apply nf_nat. apply nf_add; repeat apply ord_succ_nf; apply nf_nat. 
+  + simpl. apply head_lt. apply ord_lt_self.
+  + apply single_nf. apply nf_nat.
+- apply (ord_incr _ _  (ord_succ (ord_add (ord_succ (ord_succ (cons (nat_ord 1) 0 Zero))) (nat_ord (S m))))).
+  + unfold inductive_implication in *. unfold represent in H0. fold represent in H0. apply induction_final. unfold inductive_chain. fold inductive_chain. apply associativity2. apply associativity2. apply exchange2. apply exchange1. apply weakening.
     * simpl. repeat rewrite closed_univ_sub; auto; try apply repr_closed; simpl; rewrite H; rewrite eq_nat_refl; destruct (closed A); auto.
-    * repeat apply associativity1. apply exchange1. apply weakening; auto. simpl. rewrite (free_list_sub_self _ _ (var n)). rewrite H. simpl. rewrite eq_nat_refl. case (closed A); case (closed (substitution A n (succ (var n)))); auto. rewrite H. simpl. rewrite eq_nat_refl. auto.
-- simpl. apply head_lt. apply ord_lt_self.
-- apply w_tower_nf. 
+    * apply associativity1. apply associativity1. apply exchange1. apply weakening; auto. simpl. rewrite (free_list_sub_self _ _ (var n)). rewrite H. simpl. rewrite eq_nat_refl. case (closed A); case (closed (substitution A n (succ (var n)))); auto. rewrite H. simpl. rewrite eq_nat_refl. auto.
+  + simpl. apply coeff_lt. lia.
+  + apply single_nf. apply nf_nat. 
 Qed.
 
-Lemma induction_aux' : forall A n m, closed A = true -> PA_omega_theorem (lor (substitution A n (represent m)) (lor (neg (substitution A n zero)) (neg (univ n (lor (neg A) (substitution A n (succ (var n)))))))) 0 (w_tower (S (S (S (num_conn A + num_conn A))))).
+Lemma induction_aux' : forall A n m, closed A = true -> PA_omega_theorem (lor (substitution A n (represent m)) (lor (neg (substitution A n zero)) (neg (univ n (lor (neg A) (substitution A n (succ (var n)))))))) 0 (cons (nat_ord 1) 1 Zero).
 Proof.
-intros. pose proof (inductive_implication_theorem' _ n m H). apply (ord_incr _ _  (ord_succ (ord_add (ord_succ (ord_succ (w_tower (S (S (num_conn A + num_conn A)))))) (nat_ord (S m))))).
+intros. pose proof (inductive_implication_theorem' _ n m H). apply (ord_incr _ _  (ord_succ (cons (nat_ord 1) 0 Zero))). 
 - destruct m.
-  + apply exchange1. apply exchange3. apply associativity2. apply weakening; auto. simpl. rewrite closed_subst_eq; auto. rewrite H. simpl. auto. unfold inductive_implication in H0. repeat rewrite closed_subst_eq; auto. rewrite closed_subst_eq in H0; auto. rewrite ord_add_one_succ. apply exchange1. apply (ord_incr _ _ _ _ H0). simpl. apply tail_lt. apply zero_lt. repeat apply ord_succ_nf. apply w_tower_nf. repeat apply ord_succ_nf. apply w_tower_nf.
-  + repeat rewrite closed_subst_eq; auto. apply associativity1. apply exchange1. apply weakening. simpl. rewrite H. simpl. auto. apply exchange1. apply (ord_incr _ _ _ _ (LEM _ H)). apply (lt_trans _ _ _ (w_tower_succ _)). simpl. apply ord_lt_self. apply nf_add. repeat apply ord_succ_nf. apply w_tower_nf. apply nf_nat.
--  simpl. apply head_lt. apply ord_lt_self.
-- apply w_tower_nf. 
+  + apply exchange1. apply exchange3. apply associativity2. apply weakening; auto. simpl. rewrite closed_subst_eq; auto. rewrite H. simpl. auto. unfold inductive_implication in H0. repeat rewrite closed_subst_eq; auto. rewrite closed_subst_eq in H0; auto. apply exchange1. auto.
+  + repeat rewrite closed_subst_eq; auto. apply associativity1. apply exchange1. apply weakening. simpl. rewrite H. simpl. auto. apply exchange1. apply (ord_incr _ _ _ _ (LEM _ H)). rewrite ord_succ_nat. apply nat_lt_omega. apply zero_lt. apply single_nf. apply nf_nat.
+-  apply coeff_lt. lia.
+- apply single_nf. apply nf_nat. 
 Qed.
 
 
@@ -223,7 +224,7 @@ intros A d alpha H0. induction H0.
     unfold correct_a in *. unfold correctness in *. destruct (correct_eval _ _ X). destruct (eval (closure_t s t0)). inversion H3. destruct (eval (closure_t t t0)). inversion H2. case (eq_nat (S n0) (S n)) eqn:Y. apply eq_nat_symm in Y. rewrite Y. auto. inversion X. simpl. rewrite closed_free_list_t; auto. apply closure_closed_t. auto.
   + apply (ord_incr _ _ (ord_succ Zero)). unfold "~>". rewrite closure_lor; auto. rewrite closure_lor; auto. rewrite closure_neg; auto. rewrite closure_neg; auto. apply exchange1. apply weakening. simpl. rewrite closure_closed; auto. rewrite closure_closed; auto. apply axiom.
     simpl. destruct (correctness_decid (equ (closure_t t t0) (closure_t s t0))). simpl. rewrite closure_closed_t; auto. rewrite closure_closed_t; auto. rewrite e in X. inversion X. rewrite closure_type_equiv; auto.
-    apply ord_lt_succ. apply zero_lt. apply ord_succ_nf. apply ord_succ_nf. apply w_tower_nf.
+    apply ord_lt_succ. apply zero_lt. apply ord_succ_nf. apply ord_succ_nf. apply nf_nat.
 - intros. case (correct_a (equ (closure_t t t0) (closure_t s t0))) eqn:X. 
   + unfold "~>". rewrite closure_lor; auto. rewrite closure_neg; auto. 
     apply weakening. apply closure_closed; auto. apply axiom. rewrite closure_type_equiv; auto. simpl.
@@ -241,12 +242,15 @@ intros A d alpha H0. induction H0.
 - intros. apply axiom. rewrite closure_type_equiv; auto. rewrite closure_t_times; auto. rewrite (closure_closed_id_t zero); auto. simpl. destruct (correctness_decid (equ (times (closure_t t t0) zero) zero)); simpl; auto. rewrite closure_closed_t; auto. unfold incorrect_a in e. unfold correct_a. unfold correctness in *. simpl in *. destruct (eval (closure_t t t0)). inversion e. simpl in *. rewrite mult_0_r. rewrite eq_nat_refl. auto.
 - intros. apply axiom. rewrite closure_type_equiv; auto. rewrite closure_t_times; auto. rewrite closure_t_plus; auto. rewrite closure_t_times; auto. rewrite closure_t_succ; auto. simpl. destruct (correctness_decid (equ (times (closure_t t t0) (succ (closure_t s t0))) (plus (times (closure_t t t0) (closure_t s t0)) (closure_t t t0)))); simpl; auto. repeat rewrite closure_closed_t; auto. unfold incorrect_a in e. unfold correct_a. unfold correctness in *. simpl in *. destruct (eval (closure_t t t0)). inversion e. destruct (eval (closure_t s t0)). inversion e. assert ((S (n * S n0)) = (S (n * n0 + n))). lia. rewrite H0. rewrite eq_nat_refl. auto.
 - intros. unfold "~>". repeat rewrite closure_lor; auto. repeat rewrite closure_neg; auto. repeat rewrite closure_univ; auto. rewrite <- closure_subst; auto. rewrite closure_type_lor; auto. rewrite closure_neg_list; auto. rewrite closure_type_sub_remove; auto. case (closed (closure_type A t (free_list (univ n A)))) eqn:X.
-  + apply associativity1. apply exchange1. apply w_rule2. intros. rewrite (num_conn_closure_eq_list (free_list (univ n A)) _ t).
-    assert ( (free_list (univ n (lor (neg A) (substitution A n (succ (var n)))))) = free_list (univ n A)). simpl. case (member n (free_list A)) eqn:Y. rewrite free_list_sub_self; auto. rewrite remove_dups_concat_self. rewrite <- free_list_remove_dups. auto.
-    rewrite closed_subst_eq_aux; auto. rewrite remove_dups_concat_self. rewrite <- free_list_remove_dups. auto. rewrite H0. apply induction_aux'. auto.
+  + apply associativity1. apply exchange1. apply w_rule2. intros.
+    assert ( (free_list (univ n (lor (neg A) (substitution A n (succ (var n)))))) = free_list (univ n A)).
+    { simpl. case (member n (free_list A)) eqn:Y. rewrite free_list_sub_self; auto. rewrite remove_dups_concat_self. rewrite <- free_list_remove_dups. auto. rewrite closed_subst_eq_aux; auto. rewrite remove_dups_concat_self. rewrite <- free_list_remove_dups. auto. }
+    rewrite H0. apply induction_aux'. auto.
   + assert (free_list (closure_type A t (free_list (univ n A))) = [n]). simpl. destruct (free_list_univ_closure A _ n H); auto. apply free_list_closed in H0. rewrite H0 in X. inversion X.
-    apply associativity1. apply exchange1. apply w_rule2. intros. apply associativity1. rewrite (num_conn_closure_eq_list (free_list (univ n A)) _ t).
-    assert ( (free_list (univ n (lor (neg A) (substitution A n (succ (var n)))))) = free_list (univ n A)). simpl. case (member n (free_list A)) eqn:Y. rewrite free_list_sub_self; auto. rewrite remove_dups_concat_self. rewrite <- free_list_remove_dups. auto. rewrite closed_subst_eq_aux; auto. rewrite remove_dups_concat_self. rewrite <- free_list_remove_dups. auto. rewrite H1. apply induction_aux. auto.
+    apply associativity1. apply exchange1. apply w_rule2. intros. apply associativity1.
+    assert ( (free_list (univ n (lor (neg A) (substitution A n (succ (var n)))))) = free_list (univ n A)).
+    { simpl. case (member n (free_list A)) eqn:Y. rewrite free_list_sub_self; auto. rewrite remove_dups_concat_self. rewrite <- free_list_remove_dups. auto. rewrite closed_subst_eq_aux; auto. rewrite remove_dups_concat_self. rewrite <- free_list_remove_dups. auto. }
+    rewrite H1. apply induction_aux. auto.
 Qed.
 
 Lemma PA_Base_equiv : forall (A : formula) (d n : nat) (alpha : ord) (t : term), closed_t t = true -> Peano_Theorems_Base A d alpha -> Peano_Theorems_Base (substitution A n t) d alpha.
@@ -275,7 +279,7 @@ intros. induction H0.
 - simpl. apply mlS.
 - unfold "~>". unfold substitution. fold substitution. case (eq_nat n0 n) eqn:X.
   + apply nat_eq_decid in X. destruct X. rewrite closed_subst_eq_aux. apply induct. rewrite subst_remove; auto. apply remove_not_member.
-  + rewrite (substitution_order _ _ _ zero); auto. rewrite (weak_substitution_order _ _ _ (succ (var n0))); auto. rewrite <- (num_conn_sub A n t). apply induct. simpl. rewrite X. auto. rewrite closed_free_list_t; auto. apply eq_nat_symm'. auto. apply eq_nat_symm'. auto.
+  + rewrite (substitution_order _ _ _ zero); auto. rewrite (weak_substitution_order _ _ _ (succ (var n0))); auto. apply induct. simpl. rewrite X. auto. rewrite closed_free_list_t; auto. apply eq_nat_symm'. auto. apply eq_nat_symm'. auto.
 Qed.
 
 Lemma PA_Implication_equiv : forall (A : formula) (d n : nat) (alpha : ord) (t : term), closed_t t = true -> Peano_Theorems_Implication A d alpha -> Peano_Theorems_Implication (substitution A n t) d alpha.
@@ -304,7 +308,7 @@ intros. induction H0.
 - simpl. apply I_mlS.
 - unfold "~>". unfold substitution. fold substitution. case (eq_nat n0 n) eqn:X.
   + apply nat_eq_decid in X. destruct X. rewrite closed_subst_eq_aux. apply I_induct. rewrite subst_remove; auto. apply remove_not_member.
-  + rewrite (substitution_order _ _ _ zero); auto. rewrite (weak_substitution_order _ _ _ (succ (var n0))); auto. rewrite <- (num_conn_sub A n t). apply I_induct. simpl. rewrite X. auto. rewrite closed_free_list_t; auto. apply eq_nat_symm'. auto. apply eq_nat_symm'. auto.
+  + rewrite (substitution_order _ _ _ zero); auto. rewrite (weak_substitution_order _ _ _ (succ (var n0))); auto. apply I_induct. simpl. rewrite X. auto. rewrite closed_free_list_t; auto. apply eq_nat_symm'. auto. apply eq_nat_symm'. auto.
 Qed.
 
 Lemma PA_Base_equiv_PA_Implication : forall (A : formula) (d : nat) (alpha : ord), Peano_Theorems_Base A d alpha -> Peano_Theorems_Implication A d alpha.
